pulse/lib/pulse_core/PulseCore.Atomic.fst
@@ -1,0 +1,187 @@
+module PulseCore.Atomic
+module I = PulseCore.InstantiatedSemantics
+module A = PulseCore.Action
+open PulseCore.InstantiatedSemantics
+open PulseCore.Action
+
+let stt_atomic a #obs opens pre post =
+  A.act a opens pre post
+
+let pure_equiv (p q:prop) (_:squash (p <==> q))
+  : slprop_equiv (pure p) (pure q)
+  = FStar.PropositionalExtensionality.apply p q;
+    slprop_equiv_refl (pure p)
+
+let equiv (#p #q:slprop) (pf:slprop_equiv p q)
+: squash (p == q)
+= let _ : squash (slprop_equiv p q) = FStar.Squash.return_squash pf in
+  I.slprop_equiv_elim p q
+
+let pure_trivial (p:prop) (_:squash p)
+  : squash (pure p == emp)
+  = calc (==) {
+      pure p;
+    (==) { equiv (pure_equiv p True ()) }
+      pure True;
+    (==) { equiv (A.pure_true ()) }
+      emp;
+  }
+
+let emp_unit_r (p:slprop)
+: squash (p ** emp == p)
+= calc (==) {
+    (p ** emp);
+   (==) { equiv (slprop_equiv_comm p emp) }
+    (emp ** p);
+   (==) { equiv (slprop_equiv_unit p) }
+     p;
+  }
+
+let return_atomic' #a x post
+: stt_atomic a #Unobservable emp_inames
+      (post x ** pure (x == x))
+      (fun r -> post r ** pure (r == x))
+= A.return #a #(fun r -> post r ** pure (r == x)) x
+
+let return_atomic #a x post
+: stt_atomic a #Unobservable emp_inames
+      (post x)
+      (fun r -> post r ** pure (r == x))
+= emp_unit_r (post x);
+  pure_trivial (x == x) ();
+  coerce_eq () (return_atomic' #a x post)
+
+let bind_atomic
+    (#a:Type u#a)
+    (#b:Type u#b)
+    (#obs1:_)
+    (#obs2:observability { at_most_one_observable obs1 obs2 })
+    (#opens:inames)
+    (#pre1:slprop)
+    (#post1:a -> slprop)
+    (#post2:b -> slprop)
+    (e1:stt_atomic a #obs1 opens pre1 post1)
+    (e2:(x:a -> stt_atomic b #obs2 opens (post1 x) post2))
+= A.bind e1 e2
+
+let lift_atomic0
+    (#a:Type u#0)
+    (#obs:_)
+    (#opens:inames)
+    (#pre:slprop)
+    (#post:a -> slprop)
+    (e:stt_atomic a #obs opens pre post)
+: stt a pre post
+= A.lift0 e
+
+let lift_atomic1
+    (#a:Type u#1)
+    (#obs:_)
+    (#opens:inames)
+    (#pre:slprop)
+    (#post:a -> slprop)
+    (e:stt_atomic a #obs opens pre post)
+: stt a pre post
+= A.lift1 e
+
+let lift_atomic2
+    (#a:Type u#2)
+    (#obs:_)
+    (#opens:inames)
+    (#pre:slprop)
+    (#post:a -> slprop)
+    (e:stt_atomic a #obs opens pre post)
+: stt a pre post
+= A.lift2 e
+
+let frame_atomic
+    (#a:Type u#a)
+    (#obs: observability)
+    (#opens:inames)
+    (#pre:slprop)
+    (#post:a -> slprop)
+    (frame:slprop)
+    (e:stt_atomic a #obs opens pre post)
+: stt_atomic a #obs opens (pre ** frame) (fun x -> post x ** frame)
+= A.frame e
+
+let sub_atomic
+    (#a:Type u#a)
+    (#obs:_)
+    (#opens:inames)
+    (#pre1:slprop)
+    (pre2:slprop)
+    (#post1:a -> slprop)
+    (post2:a -> slprop)
+    (pf1 : slprop_equiv pre1 pre2)
+    (pf2 : slprop_post_equiv post1 post2)
+    (e:stt_atomic a #obs opens pre1 post1)
+: stt_atomic a #obs opens pre2 post2
+= A.sub pre2 post2 e
+
+let sub_invs_stt_atomic
+    (#a:Type u#a)
+    (#obs:_)
+    (#opens1 #opens2:inames)
+    (#pre:slprop)
+    (#post:a -> slprop)
+    (e:stt_atomic a #obs opens1 pre post)
+    (_ : squash (inames_subset opens1 opens2))
+: stt_atomic a #obs opens2 pre post
+= assert (Set.equal (Set.union opens1 opens2) opens2);
+  A.weaken opens2 e
+
+let stt_ghost a opens pre post = Ghost.erased (act a opens pre post)
+let return_ghost #a x p = Ghost.hide (return_atomic #a x p)
+let bind_ghost
+    (#a:Type u#a)
+    (#b:Type u#b)
+    (#opens:inames)
+    (#pre1:slprop)
+    (#post1:a -> slprop)
+    (#post2:b -> slprop)
+    (e1:stt_ghost a opens pre1 post1)
+    (e2:(x:a -> stt_ghost b opens (post1 x) post2))
+: stt_ghost b opens pre1 post2
+= let e1 = Ghost.reveal e1 in
+  let e2 = FStar.Ghost.Pull.pull (fun (x:a) -> Ghost.reveal (e2 x)) in
+  Ghost.hide (A.bind e1 e2)
+
+let lift_ghost
+    (#a:Type u#a)
+    (#opens:inames)
+    (#pre:slprop)
+    (#post:a -> slprop)
+    (e:stt_ghost a opens pre post)
+    (reveal_a:non_informative_witness a)
+: stt_atomic a #Unobservable opens pre post
+= admit() //This is the main axiom about ghost computations; in Steel, this axiom is implemented within the effect system
+
+let frame_ghost
+    (#a:Type u#a)
+    (#opens:inames)
+    (#pre:slprop)
+    (#post:a -> slprop)
+    (frame:slprop)
+    (e:stt_ghost a opens pre post)
+: stt_ghost a opens (pre ** frame) (fun x -> post x ** frame)
+= Ghost.hide (A.frame (Ghost.reveal e))
+ 
+let new_invariant
+    (p:slprop)
+: stt_atomic (inv p) #Unobservable emp_inames p (fun _ -> emp)
+= A.new_invariant p
+
+let with_invariant
+    (#a:Type)
+    (#obs:_)
+    (#fp:slprop)
+    (#fp':a -> slprop)
+    (#f_opens:inames)
+    (#p:slprop)
+    (i:inv p{not (mem_inv f_opens i)})
+    ($f:unit -> stt_atomic a #obs f_opens
+                            (p ** fp)
+                            (fun x -> p ** fp' x))
+: stt_atomic a #obs (add_inv f_opens i) fp fp'
+= A.with_invariant i f
