pulse/lib/pulse_core/PulseCore.Atomic.fsti
@@ -1,0 +1,184 @@
+module PulseCore.Atomic
+open PulseCore.InstantiatedSemantics
+open PulseCore.Action
+open FStar.Ghost
+
+type observability =
+  | Observable
+  | Unobservable
+
+let at_most_one_observable o1 o2 =
+  match o1, o2 with
+  | Observable, Observable -> false
+  | _ -> true
+
+let join_obs o1 o2 =
+  match o1, o2 with
+  | Observable, _
+  | _, Observable -> Observable
+  | _ -> Unobservable
+
+(* stt_unobservable a opens pre post: The type of a pulse computation
+   that when run in a state satisfying `pre`
+   takes an unobservable atomic step
+   potentially opening invariants in `opens`
+   and returns `x:a`
+   such that the final state satisfies `post x` *)
+[@@extract_as_impure_effect]
+val stt_atomic
+    (a:Type u#a)
+    (#obs:observability)
+    (opens:inames)
+    (pre:slprop)
+    (post:a -> slprop)
+: Type u#(max 2 a)
+
+val return_atomic
+    (#a:Type u#a)
+    (x:a)
+    (p:a -> slprop)
+: stt_atomic a #Unobservable emp_inames (p x) (fun r -> p r ** pure (r == x))
+
+val bind_atomic
+    (#a:Type u#a)
+    (#b:Type u#b)
+    (#obs1:_)
+    (#obs2:observability { at_most_one_observable obs1 obs2 })
+    (#opens:inames)
+    (#pre1:slprop)
+    (#post1:a -> slprop)
+    (#post2:b -> slprop)
+    (e1:stt_atomic a #obs1 opens pre1 post1)
+    (e2:(x:a -> stt_atomic b #obs2 opens (post1 x) post2))
+: stt_atomic b #(join_obs obs1 obs2) opens pre1 post2
+
+val lift_atomic0
+    (#a:Type u#0)
+    (#obs:_)
+    (#opens:inames)
+    (#pre:slprop)
+    (#post:a -> slprop)
+    (e:stt_atomic a #obs opens pre post)
+: stt a pre post
+
+val lift_atomic1
+    (#a:Type u#1)
+    (#obs:_)
+    (#opens:inames)
+    (#pre:slprop)
+    (#post:a -> slprop)
+    (e:stt_atomic a #obs opens pre post)
+: stt a pre post
+
+val lift_atomic2
+    (#a:Type u#2)
+    (#obs:_)
+    (#opens:inames)
+    (#pre:slprop)
+    (#post:a -> slprop)
+    (e:stt_atomic a #obs opens pre post)
+: stt a pre post
+
+val frame_atomic
+    (#a:Type u#a)
+    (#obs: observability)
+    (#opens:inames)
+    (#pre:slprop)
+    (#post:a -> slprop)
+    (frame:slprop)
+    (e:stt_atomic a #obs opens pre post)
+: stt_atomic a #obs opens (pre ** frame) (fun x -> post x ** frame)
+
+val sub_atomic
+    (#a:Type u#a)
+    (#obs:_)
+    (#opens:inames)
+    (#pre1:slprop)
+    (pre2:slprop)
+    (#post1:a -> slprop)
+    (post2:a -> slprop)
+    (pf1 : slprop_equiv pre1 pre2)
+    (pf2 : slprop_post_equiv post1 post2)
+    (e:stt_atomic a #obs opens pre1 post1)
+: stt_atomic a #obs opens pre2 post2
+
+val sub_invs_stt_atomic
+    (#a:Type u#a)
+    (#obs:_)
+    (#opens1 #opens2:inames)
+    (#pre:slprop)
+    (#post:a -> slprop)
+    (e:stt_atomic a #obs opens1 pre post)
+    (_ : squash (inames_subset opens1 opens2))
+: stt_atomic a #obs opens2 pre post
+
+(* stt_ghost a opens pre post: The type of a pulse computation
+   that when run in a state satisfying `pre`
+   takes a single ghost atomic step (i.e. a step that does not modify the heap, and does not get extracted)
+   potentially opening invariants in `opens`
+   and returns `x:a`
+   such that the final state satisfies `post x` *)
+[@@ erasable]
+val stt_ghost
+    (a:Type u#a)
+    (opens:inames)
+    (pre:slprop)
+    (post:a -> slprop)
+: Type u#(max 2 a)
+
+val return_ghost
+    (#a:Type u#a)
+    (x:a)
+    (p:a -> slprop)
+: stt_ghost a emp_inames (p x) (fun r -> p r ** pure (r == x))
+
+val bind_ghost
+    (#a:Type u#a)
+    (#b:Type u#b)
+    (#opens:inames)
+    (#pre1:slprop)
+    (#post1:a -> slprop)
+    (#post2:b -> slprop)
+    (e1:stt_ghost a opens pre1 post1)
+    (e2:(x:a -> stt_ghost b opens (post1 x) post2))
+: stt_ghost b opens pre1 post2
+
+type non_informative_witness (a:Type u#a) =
+  x:Ghost.erased a -> y:a{y == Ghost.reveal x}
+
+val lift_ghost
+    (#a:Type u#a)
+    (#opens:inames)
+    (#pre:slprop)
+    (#post:a -> slprop)
+    (e:stt_ghost a opens pre post)
+    (reveal_a:non_informative_witness a)
+: stt_atomic a #Unobservable opens pre post
+
+val frame_ghost
+    (#a:Type u#a)
+    (#opens:inames)
+    (#pre:slprop)
+    (#post:a -> slprop)
+    (frame:slprop)
+    (e:stt_ghost a opens pre post)
+: stt_ghost a opens (pre ** frame) (fun x -> post x ** frame)
+ 
+//////////////////////////////////////////////////////////////////
+
+val new_invariant
+    (p:slprop)
+: stt_atomic (inv p) #Unobservable emp_inames p (fun _ -> emp)
+
+val with_invariant
+    (#a:Type)
+    (#obs:_)
+    (#fp:slprop)
+    (#fp':a -> slprop)
+    (#f_opens:inames)
+    (#p:slprop)
+    (i:inv p{not (mem_inv f_opens i)})
+    ($f:unit -> stt_atomic a #obs f_opens
+                            (p ** fp)
+                            (fun x -> p ** fp' x))
+: stt_atomic a #obs (add_inv f_opens i) fp fp'
